Impl/DiskOpModel.i.dfy
@@ -1,10 +1,19 @@
 include "../ByteBlockCacheSystem/AsyncDiskModel.s.dfy"
+include "../BlockCacheSystem/BlockJournalCache.i.dfy"
 
 module DiskOpModel {
   import D = AsyncDisk
   import opened NativeTypes
+  import BJC = BlockJournalCache
+  import BC = BlockCache
+  import JC = JournalCache
 
   datatype Constants = Constants()
+
+  function Ik(k: Constants) : BJC.Constants
+  {
+    BJC.Constants(BC.Constants(), JC.Constants())
+  }
 
   // Functional model of the DiskIOHandler
 
